change notation

03_Fixpoint_Earley_Recognizer.thy
@@ -32,10 +32,10 @@ Non-recursive definitions are introduced with the \textit{definition} keyword.
 
 It is standard to define a language as a set of strings over a finite set of symbols. We deviate slightly by introducing a type variable $'a$
 for the type of symbols. Thus a string corresponds to a list of symbols and a language is formalized as
-a set of lists of symbols. We represent a context-free grammar as the datatype @{term CFG}. An instance \textit{cfg} consists of (1) a list of
-non-terminals (@{term "\<NN> cfg"}), (2) a list of terminals (@{term "\<TT> cfg"}), (3) a list of production rules
-(@{term "\<RR> cfg"}), and a start symbol (@{term "\<SS> cfg"}) where @{term \<NN>}, @{term \<TT>}, @{term \<RR>} and @{term \<SS>} are
-projections accessing the specific part of an instance @{term cfg} of the datatype @{term CFG}. Each rule consists of a left-hand side or @{term rule_head}, a single symbol,
+a set of lists of symbols. We represent a context-free grammar as the datatype @{term CFG}. An instance @{term \<G>} consists of (1) a list of
+non-terminals (@{term "\<NN> \<G>"}), (2) a list of terminals (@{term "\<TT> \<G>"}), (3) a list of production rules
+(@{term "\<RR> \<G>"}), and a start symbol (@{term "\<SS> \<G>"}) where @{term \<NN>}, @{term \<TT>}, @{term \<RR>} and @{term \<SS>} are
+projections accessing the specific part of an instance @{term \<G>} of the datatype @{term CFG}. Each rule consists of a left-hand side or @{term rule_head}, a single symbol,
 and a right-hand side or @{term rule_body}, a list of symbols.
 The productions with a particular non-terminal $N$ on their left-hand sides are called the alternatives of $N$.
 We make the usual assumptions about the well-formedness of a context-free grammar: the intersection of the set of terminals and
@@ -61,23 +61,45 @@ definition rule_body :: "'a rule \<Rightarrow> 'a list" where
   "rule_body = snd"
 
 definition disjunct_symbols :: "'a cfg \<Rightarrow> bool" where
-  "disjunct_symbols cfg \<equiv> set (\<NN> cfg) \<inter> set (\<TT> cfg) = {}"
+  "disjunct_symbols \<G> \<equiv> set (\<NN> \<G>) \<inter> set (\<TT> \<G>) = {}"
 
 definition wf_startsymbol :: "'a cfg \<Rightarrow> bool" where
-  "wf_startsymbol cfg \<equiv> \<SS> cfg \<in> set (\<NN> cfg)"
+  "wf_startsymbol \<G> \<equiv> \<SS> \<G> \<in> set (\<NN> \<G>)"
 
 definition wf_rules :: "'a cfg \<Rightarrow> bool" where
-  "wf_rules cfg \<equiv> \<forall>(N, \<alpha>) \<in> set (\<RR> cfg). N \<in> set (\<NN> cfg) \<and> (\<forall>s \<in> set \<alpha>. s \<in> set (\<NN> cfg) \<union> set (\<TT> cfg))"
+  "wf_rules \<G> \<equiv> \<forall>(N, \<alpha>) \<in> set (\<RR> \<G>). N \<in> set (\<NN> \<G>) \<and> (\<forall>s \<in> set \<alpha>. s \<in> set (\<NN> \<G>) \<union> set (\<TT> \<G>))"
 
 definition distinct_rules :: "'a cfg \<Rightarrow> bool" where
-  "distinct_rules cfg \<equiv> distinct (\<RR> cfg)"
+  "distinct_rules \<G> \<equiv> distinct (\<RR> \<G>)"
 
-definition wf_cfg :: "'a cfg \<Rightarrow> bool" where
-  "wf_cfg cfg \<equiv> disjunct_symbols cfg \<and> wf_startsymbol cfg \<and> wf_rules cfg \<and> distinct_rules cfg"
+definition wf_\<G> :: "'a cfg \<Rightarrow> bool" where
+  "wf_\<G> \<G> \<equiv> disjunct_symbols \<G> \<and> wf_startsymbol \<G> \<and> wf_rules \<G> \<and> distinct_rules \<G>"
+
+(*<*)
+(*
+notation
+  derives1 ("_ \<turnstile> _ \<Rightarrow> _" [1000,0] 1000)
+
+notation
+  derives ("_ \<turnstile> _ \<^latex>\<open>\\ensuremath{\\xRightarrow{\\ast}}\<close> _" [1000,0] 1000)
+
+notation
+  slice ("_\<^latex>\<open>[\<close>_\<^latex>\<open>..\<close>_\<^latex>\<open>)\<close>" [1000,0] 1000)
+*)
+
+syntax
+  "derives1" :: "'a cfg \<Rightarrow> 'a list \<Rightarrow> 'a list \<Rightarrow> bool" ("_ \<turnstile> _ \<Rightarrow> _" [1000,0] 1000)
+
+syntax
+  "derives" :: "'a cfg \<Rightarrow> 'a list \<Rightarrow> 'a list \<Rightarrow> bool" ("_ \<turnstile> _ \<Rightarrow>\<^sup>* _" [1000,0] 1000)
+
+syntax
+  "slice" :: "'a list \<Rightarrow> nat \<Rightarrow> nat \<Rightarrow> 'a list" ("_[_.. _\<rangle>" [1000,0] 1000)
+(*>*)
 
 text\<open>
 Furthermore, in Isabelle, lists are constructed from the empty list @{term "[]"} via the infix cons-operator @{term "(#)"};
-the operator @{term "(@)"} appends two lists; @{term "xs!n"} returns the $n$-th item of the list @{term xs}.
+the operator @{term "(@)"} appends two lists; @{term "|xs|"} denotes the length and @{term "xs!n"} returns the $n$-th item of the list @{term xs}.
 Sets follow the standard mathematical notation including
 the commonly found set builder notation or set comprehensions @{term "{ x | x. P x}"}. Sets can also be defined
 inductively using the keyword \textit{inductive\_set}.
@@ -85,65 +107,61 @@ inductively using the keyword \textit{inductive\_set}.
 Next we formalize the concept of a derivation. We use lowercase letters $a$, $b$, $c$ indicating terminal symbols; capital letters
 $A$, $B$, $C$ denote non-terminals; lists of symbols are represented by greek letters: \alpha, \beta, \gamma, occasionally also by lowercase letters $u$, $v$, $w$.
 The empty list in the context of a language is \epsilon. A sentential is a list consisting of only symbols. A sentence
-is a sentential if it only contains terminal symbols. We first define a predicate @{term "derives1 cfg u v"} which expresses that
+is a sentential if it only contains terminal symbols. We first define a predicate @{term "derives1 \<G> u v"} which expresses that
 we can derive $v$ from $u$ in a single step or the predicate holds if there exist $\alpha$, $\beta$, $N$ and $\gamma$ such that @{term "u = \<alpha> @ [N] @ \<beta>"},
-@{term "v = \<alpha> @ \<gamma> @ \<beta>"} and @{term "(N, \<gamma>)"} is a production rule. We then can define the set of single-step derivations using @{term derives1},
+@{term "v = \<alpha> @ \<gamma> @ \<beta>"} and @{term "(N, \<gamma>)"} is a production rule. We also introduce more convenient notation: @{term "derives1 \<G> u v"} is written @{term \<G>} $\vdash u \Rightarrow v$ We then can define the set of single-step derivations using @{term derives1},
 and subsequently the set of all derivations given a particular grammar is the reflexive-transitive closure of the set of
-single-step derivations. Finally, we say $v$ can be derived from $u$ given a grammar \textit{cfg}, or @{term "derives cfg u v"} if
-@{term "(u, v) \<in> derivations cfg"}.
+single-step derivations. Finally, we say $v$ can be derived from $u$ given a grammar @{term \<G>} or @{term "derives \<G> u v"} if
+@{term "(u, v) \<in> derivations \<G>"}. The more convenient notation is again: @{term "derives \<G> u v"} $=$ @{term \<G>} $\vdash u \Rightarrow^{\ast} v$
 \<close>
 
 type_synonym 'a sentential = "'a list"
 
 definition is_terminal :: "'a cfg \<Rightarrow> 'a \<Rightarrow> bool" where
-  "is_terminal cfg s \<equiv> s \<in> set (\<TT> cfg)"
+  "is_terminal \<G> s \<equiv> s \<in> set (\<TT> \<G>)"
 
 definition is_nonterminal :: "'a cfg \<Rightarrow> 'a \<Rightarrow> bool" where
-  "is_nonterminal cfg s \<equiv> s \<in> set (\<NN> cfg)"
+  "is_nonterminal \<G> s \<equiv> s \<in> set (\<NN> \<G>)"
 
 definition is_symbol :: "'a cfg \<Rightarrow> 'a \<Rightarrow> bool" where
-  "is_symbol cfg s \<equiv> is_terminal cfg s \<or> is_nonterminal cfg s"
+  "is_symbol \<G> s \<equiv> is_terminal \<G> s \<or> is_nonterminal \<G> s"
 
 definition wf_sentential :: "'a cfg \<Rightarrow> 'a sentential \<Rightarrow> bool" where
-  "wf_sentential cfg s \<equiv> \<forall>x \<in> set s. is_symbol cfg x"
+  "wf_sentential \<G> s \<equiv> \<forall>x \<in> set s. is_symbol \<G> x"
 
 definition is_sentence :: "'a cfg \<Rightarrow> 'a sentential \<Rightarrow> bool" where
-  "is_sentence cfg s \<equiv> \<forall>x \<in> set s. is_terminal cfg x"
-
-\<comment>\<open>TODO\<close>
-(*<*)
-notation (latex output)
-  nth  ("_\<^latex>\<open>\\ensuremath{_{[\\mathit{\<close>_\<^latex>\<open>}]}}\<close>" [1000,0] 1000)
-(*>*)
+  "is_sentence \<G> s \<equiv> \<forall>x \<in> set s. is_terminal \<G> x"
 
 definition derives1 :: "'a cfg \<Rightarrow> 'a sentential \<Rightarrow> 'a sentential \<Rightarrow> bool" where
-  "derives1 cfg u v \<equiv>
+  "derives1 \<G> u v \<equiv>
      \<exists> \<alpha> \<beta> N \<gamma>. 
          u = \<alpha> @ [N] @ \<beta>
        \<and> v = \<alpha> @ \<gamma> @ \<beta>
-       \<and> (N, \<gamma>) \<in> set (\<RR> cfg)"  
+       \<and> (N, \<gamma>) \<in> set (\<RR> \<G>)"
+
 
 definition derivations1 :: "'a cfg \<Rightarrow> ('a sentential \<times> 'a sentential) set" where
-  "derivations1 cfg = { (u,v) | u v. derives1 cfg u v }"
+  "derivations1 \<G> = { (u,v) | u v. \<G> \<turnstile> u \<Rightarrow> v }"
 
 definition derivations :: "'a cfg \<Rightarrow> ('a sentential \<times> 'a sentential) set" where 
-  "derivations cfg = (derivations1 cfg)^*"
+  "derivations \<G> = (derivations1 \<G>)^*"
 
 definition derives :: "'a cfg \<Rightarrow> 'a sentential \<Rightarrow> 'a sentential \<Rightarrow> bool" where
-  "derives cfg u v \<equiv> (u, v) \<in> derivations cfg"
+  "derives \<G> u v \<equiv> (u, v) \<in> derivations \<G>"
 
 text\<open>
 Potentially recursive but provably total functions that may make use of pattern matching are defined with
 the \textit{fun} and \textit{function} keywords; partial functions are defined via \textit{partial\_function}.
-Take for example the function @{term slice} defined below. Term @{term "slice i j xs"} computes the slice of a list @{term xs}
-between indices $i$ (inclusive) and $j$ (exclusive), e.g. @{term "slice (2::nat) (4::nat) [a, b, c, d, e]"} evaluates to @{term "[c, d]"}.
+Take for example the function @{term slice} defined below. Term @{term "slice xs i j"} computes the slice of a list @{term xs}
+between indices $i$ (inclusive) and $j$ (exclusive), e.g. @{term "slice [a, b, c, d, e] (2::nat) (4::nat)"} evaluates to @{term "[c, d]"}.
+We also introduce a shorthand notation: e.g. @{term "slice xs i j"} is written @{term "xs"}$[ i..j \rangle$.
 \<close>
 
-fun slice :: "nat \<Rightarrow> nat \<Rightarrow> 'a list \<Rightarrow> 'a list" where
-  "slice _ _ [] = []"
-| "slice _ 0 (x#xs) = []"
-| "slice 0 (Suc b) (x#xs) = x # slice 0 b xs"
-| "slice (Suc a) (Suc b) (x#xs) = slice a b xs"
+fun slice :: "'a list \<Rightarrow> nat \<Rightarrow> nat \<Rightarrow> 'a list" where
+  "slice [] _ _ = []"
+| "slice (x#xs) _ 0  = []"
+| "slice (x#xs) 0 (Suc b) = x # slice xs 0 b"
+| "slice (x#xs) (Suc a) (Suc b) = slice xs a b"
 
 text\<open>
 Lemmas, theorems and corollaries are presented using the keywords \textit{lemma}, \textit{theorem}, \textit{corollary} respectively, followed
@@ -154,7 +172,7 @@ and the append operator @{term "(@)"}, stating the conditions under which we can
 
 lemma slice_append:
   assumes "i \<le> j" "j \<le> k"
-  shows "slice i j xs @ slice j k xs = slice i k xs"
+  shows "xs[i..j\<rangle> @ xs[j..k\<rangle> = xs[i..k\<rangle>"
 (*<*)
   sorry
 (*>*)
@@ -172,7 +190,7 @@ of an item. Functions @{term item_\<alpha>} and @{term item_\<beta>} split the p
 We call an item @{term complete} if the bullet is at the end of the production rule body. The next symbol (@{term next_symbol}) of
 an item is either @{term None} if it is complete, or @{term "Some s"} where $s$ is the symbol in the production
 rule body following the bullet. An item is finished if the item rule head is the start symbol, the item is complete, and
-the whole input has been scanned or @{term "item_origin item = (0::nat)"} and @{term "item_end item = length \<omega>"}. Finally, we call a set of
+the whole input has been scanned or @{term "item_origin item = (0::nat)"} and @{term "item_end item = |\<omega>|"}. Finally, we call a set of
 items @{term recognizing} if it contains at least one finished item, indicating that this set of items recognizes the input $\omega$.
 \<close>
 
@@ -198,20 +216,20 @@ definition item_\<beta> :: "'a item \<Rightarrow> 'a sentential" where
   "item_\<beta> x = drop (item_bullet x) (item_rule_body x)"
 
 definition is_complete :: "'a item \<Rightarrow> bool" where
-  "is_complete x \<equiv> item_bullet x \<ge> length (item_rule_body x)"
+  "is_complete x \<equiv> item_bullet x \<ge> |item_rule_body x|"
 
 definition next_symbol :: "'a item \<Rightarrow> 'a option" where
-  "next_symbol x \<equiv> if is_complete x then None else Some ((item_rule_body x) ! (item_bullet x))"
+  "next_symbol x \<equiv> if is_complete x then None else Some (item_rule_body x ! item_bullet x)"
 
 definition is_finished :: "'a cfg \<Rightarrow> 'a sentential \<Rightarrow> 'a item \<Rightarrow> bool" where
-  "is_finished cfg \<omega> x \<equiv> 
-    item_rule_head x = \<SS> cfg \<and>
+  "is_finished \<G> \<omega> x \<equiv> 
+    item_rule_head x = \<SS> \<G> \<and>
     item_origin x = 0 \<and>
-    item_end x = length \<omega> \<and> 
+    item_end x = |\<omega>| \<and> 
     is_complete x"
 
 definition recognizing :: "'a items \<Rightarrow> 'a cfg \<Rightarrow> 'a sentential \<Rightarrow> bool" where
-  "recognizing I cfg \<omega> \<equiv> \<exists>x \<in> I. is_finished cfg \<omega> x"
+  "recognizing I \<G> \<omega> \<equiv> \<exists>x \<in> I. is_finished \<G> \<omega> x"
 
 text\<open>
 Normally we don't construct items directly via the @{term Item} constructor but use two auxiliary constructors:
@@ -252,20 +270,20 @@ definition bin :: "'a items \<Rightarrow> nat \<Rightarrow> 'a items" where
   "bin I k = { x . x \<in> I \<and> item_end x = k }"
 
 definition Init :: "'a cfg \<Rightarrow> 'a items" where
-  "Init cfg = { init_item r 0 | r. r \<in> set (\<RR> cfg) \<and> fst r = (\<SS> cfg) }"
+  "Init \<G> = { init_item r 0 | r. r \<in> set (\<RR> \<G>) \<and> fst r = (\<SS> \<G>) }"
 
 definition Scan :: "nat \<Rightarrow> 'a sentential \<Rightarrow> 'a items \<Rightarrow> 'a items" where
   "Scan k \<omega> I = 
     { inc_item x (k+1) | x a.
         x \<in> bin I k \<and>
         \<omega>!k = a \<and>
-        k < length \<omega> \<and>
+        k < |\<omega>| \<and>
         next_symbol x = Some a }"
 
 definition Predict :: "nat \<Rightarrow> 'a cfg \<Rightarrow> 'a items \<Rightarrow> 'a items" where
-  "Predict k cfg I =
+  "Predict k \<G> I =
     { init_item r k | r x.
-        r \<in> set (\<RR> cfg) \<and>
+        r \<in> set (\<RR> \<G>) \<and>
         x \<in> bin I k \<and>
         next_symbol x = Some (rule_head r) }"
 
@@ -278,7 +296,7 @@ definition Complete :: "nat \<Rightarrow> 'a items \<Rightarrow> 'a items" where
         next_symbol x = Some (item_rule_head y) }"
 
 definition Earley_step :: "nat \<Rightarrow> 'a cfg \<Rightarrow> 'a sentential \<Rightarrow> 'a items \<Rightarrow> 'a items" where
-  "Earley_step k cfg \<omega> I = I \<union> Scan k \<omega> I \<union> Complete k I \<union> Predict k cfg I"
+  "Earley_step k \<G> \<omega> I = I \<union> Scan k \<omega> I \<union> Complete k I \<union> Predict k \<G> I"
 
 fun funpower :: "('a \<Rightarrow> 'a) \<Rightarrow> nat \<Rightarrow> ('a \<Rightarrow> 'a)" where
   "funpower f 0 x = x"
@@ -291,14 +309,14 @@ definition limit :: "('a set \<Rightarrow> 'a set) \<Rightarrow> 'a set \<Righta
   "limit f x = natUnion (\<lambda> n. funpower f n x)"
 
 definition Earley_bin :: "nat \<Rightarrow> 'a cfg \<Rightarrow> 'a sentential \<Rightarrow> 'a items \<Rightarrow> 'a items" where
-  "Earley_bin k cfg \<omega> I = limit (Earley_step k cfg \<omega>) I"
+  "Earley_bin k \<G> \<omega> I = limit (Earley_step k \<G> \<omega>) I"
 
 fun Earley :: "nat \<Rightarrow> 'a cfg \<Rightarrow> 'a sentential \<Rightarrow> 'a items" where
-  "Earley 0 cfg \<omega> = Earley_bin 0 cfg \<omega> (Init cfg)"
-| "Earley (Suc n) cfg \<omega> = Earley_bin (Suc n) cfg \<omega> (Earley n cfg \<omega>)"
+  "Earley 0 \<G> \<omega> = Earley_bin 0 \<G> \<omega> (Init \<G>)"
+| "Earley (Suc n) \<G> \<omega> = Earley_bin (Suc n) \<G> \<omega> (Earley n \<G> \<omega>)"
 
 definition \<E>arley :: "'a cfg \<Rightarrow> 'a sentential \<Rightarrow> 'a items" where
-  "\<E>arley cfg \<omega> = Earley (length \<omega>) cfg \<omega>"
+  "\<E>arley \<G> \<omega> = Earley |\<omega>| \<G> \<omega>"
 
 text\<open>
 We follow the operational approach of defining the set of Earley items primarily for two reasons: first of all, we reuse and only slightly adapt
@@ -331,17 +349,17 @@ finally the item end is at most the length of the input.
 \<close>
 
 definition wf_item :: "'a cfg \<Rightarrow> 'a sentential => 'a item \<Rightarrow> bool" where 
-  "wf_item cfg \<omega> x \<equiv> 
-    item_rule x \<in> set (\<RR> cfg) \<and> 
-    item_bullet x \<le> length (item_rule_body x) \<and>
+  "wf_item \<G> \<omega> x \<equiv> 
+    item_rule x \<in> set (\<RR> \<G>) \<and> 
+    item_bullet x \<le> |item_rule_body x| \<and>
     item_origin x \<le> item_end x \<and> 
-    item_end x \<le> length \<omega>"
+    item_end x \<le> |\<omega>|"
 
 definition wf_items :: "'a cfg \<Rightarrow> 'a sentential \<Rightarrow> 'a items \<Rightarrow> bool" where
-  "wf_items cfg \<omega> I \<equiv> \<forall>x \<in> I. wf_item cfg \<omega> x"
+  "wf_items \<G> \<omega> I \<equiv> \<forall>x \<in> I. wf_item \<G> \<omega> x"
 
 lemma wf_Init:
-  shows "wf_items cfg \<omega> (Init cfg)"
+  shows "wf_items \<G> \<omega> (Init \<G>)"
 (*<*)
   sorry
 (*>*)
@@ -349,8 +367,8 @@ lemma wf_Init:
 text\<open>\<close>
 
 lemma wf_Scan_Predict_Complete:
-  assumes "wf_items cfg \<omega> I" 
-  shows "wf_items cfg \<omega> (Scan k \<omega> I \<union> Predict k cfg I \<union> Complete k I)"
+  assumes "wf_items \<G> \<omega> I" 
+  shows "wf_items \<G> \<omega> (Scan k \<omega> I \<union> Predict k \<G> I \<union> Complete k I)"
 (*<*)
   sorry
 (*>*)
@@ -358,8 +376,8 @@ lemma wf_Scan_Predict_Complete:
 text\<open>\<close>
 
 lemma wf_Earley_step:
-  assumes "wf_items cfg \<omega> I"
-  shows "wf_items cfg \<omega> (Earley_step k cfg \<omega> I)"
+  assumes "wf_items \<G> \<omega> I"
+  shows "wf_items \<G> \<omega> (Earley_step k \<G> \<omega> I)"
 (*<*)
   sorry
 (*>*)
@@ -370,8 +388,8 @@ follow trivially by definition of the respective operations.
 \<close>
 
 lemma wf_funpower:
-  assumes "wf_items cfg \<omega> I"
-  shows "wf_items cfg \<omega> (funpower (Earley_step k cfg \<omega>) n I)"
+  assumes "wf_items \<G> \<omega> I"
+  shows "wf_items \<G> \<omega> (funpower (Earley_step k \<G> \<omega>) n I)"
 (*<*)
   sorry
 (*>*)
@@ -379,8 +397,8 @@ lemma wf_funpower:
 text\<open>\<close>
 
 lemma wf_Earley_bin:
-  assumes "wf_items cfg \<omega> I"
-  shows "wf_items cfg \<omega> (Earley_bin k cfg \<omega> I)"
+  assumes "wf_items \<G> \<omega> I"
+  shows "wf_items \<G> \<omega> (Earley_bin k \<G> \<omega> I)"
 (*<*)
   sorry
 (*>*)
@@ -388,7 +406,7 @@ lemma wf_Earley_bin:
 text\<open>\<close>
 
 lemma wf_Earley_bin0:
-  shows "wf_items cfg \<omega> (Earley_bin 0 cfg \<omega> (Init cfg))"
+  shows "wf_items \<G> \<omega> (Earley_bin 0 \<G> \<omega> (Init \<G>))"
 (*<*)
   sorry
 (*>*)
@@ -400,7 +418,7 @@ that @{term "x \<in> limit f X \<equiv> \<exists>n. x \<in> funpower f n X"} and
 \<close>
 
 lemma wf_Earley:
-  shows "wf_items cfg \<omega> (Earley n cfg \<omega>)"
+  shows "wf_items \<G> \<omega> (Earley n \<G> \<omega>)"
 (*<*)
   sorry
 (*>*)
@@ -408,7 +426,7 @@ lemma wf_Earley:
 text\<open>\<close>
 
 lemma wf_\<E>arley:
-  shows "wf_items cfg \<omega> (\<E>arley cfg \<omega>)"
+  shows "wf_items \<G> \<omega> (\<E>arley \<G> \<omega>)"
 (*<*)
   sorry
 (*>*)
@@ -430,42 +448,62 @@ about derivations.
 \<close>
 
 definition sound_item :: "'a cfg \<Rightarrow> 'a sentential \<Rightarrow> 'a item \<Rightarrow> bool" where
-  "sound_item cfg \<omega> x = derives cfg [item_rule_head x] (slice (item_origin x) (item_end x) \<omega> @ item_\<beta> x)"
+  "sound_item \<G> \<omega> x = \<G> \<turnstile> [item_rule_head x] \<Rightarrow>\<^sup>* \<omega>[item_origin x..item_end x\<rangle> @ item_\<beta> x"
 
 definition sound_items :: "'a cfg \<Rightarrow> 'a sentential \<Rightarrow> 'a items \<Rightarrow> bool" where
-  "sound_items cfg \<omega> I \<equiv> \<forall>x \<in> I. sound_item cfg \<omega> x"
+  "sound_items \<G> \<omega> I \<equiv> \<forall>x \<in> I. sound_item \<G> \<omega> x"
 
 text\<open>
 Obua \cite{Obua:2017} \cite{LocalLexing-AFP} defines derivations at two different abstraction levels.
 The first representation is as the reflexive-transitive closure of the set of one-step derivations as introduced earlier in this chapter.
-The second representation is again more operational. He defines a predicate @{term "Derives1 cfg u i r v"}
-that is conceptually analogous to the predicate @{term "derives1 cfg u v"} but also captures the rule $r$
+The second representation is again more operational. He defines a predicate @{term "Derives1 \<G> u i r v"}
+that is conceptually analogous to the predicate @{term "\<G> \<turnstile> u \<Rightarrow> v"} but also captures the rule $r$
 used for a single rewriting step and the position $i$ in $u$ where the rewriting occurs.
 \<close>
 
+(*<*)
+syntax
+  "Derives1" :: "'a cfg \<Rightarrow> 'a sentential \<Rightarrow> nat \<Rightarrow> 'a rule \<Rightarrow> 'a sentential \<Rightarrow> bool" ("_ \<turnstile> _ \<Rightarrow>(_, _) _" [1000,0] 1000)
+(*>*)
+
 definition Derives1 :: "'a cfg \<Rightarrow> 'a sentential \<Rightarrow> nat \<Rightarrow> 'a rule \<Rightarrow> 'a sentential \<Rightarrow> bool" where
-  "Derives1 cfg u i r v \<equiv> 
+  "Derives1 \<G> u i r v \<equiv> 
      \<exists> \<alpha> \<beta> N \<gamma>. 
           u = \<alpha> @ [N] @ \<beta>
         \<and> v = \<alpha> @ \<gamma> @ \<beta>
-        \<and> (N, \<gamma>) \<in> set (\<RR> cfg)
-        \<and> r = (N, \<gamma>) \<and> i = length \<alpha>"
+        \<and> (N, \<gamma>) \<in> set (\<RR> \<G>)
+        \<and> r = (N, \<gamma>) \<and> i = |\<alpha>|"
 
 text\<open>
 He then defines the type of a \textit{derivation} as a list of pairs representing precisely the positions and rules
 used to apply each rewrite step. The predicate @{term Derivation} is defined recursively as follows: @{term "Derivation \<alpha> [] \<beta>"} holds only if @{term "\<alpha> = \<beta>"}. If the derivation consists of at least one rewrite pair $(i, r)$, or
-@{term "Derivation cfg \<alpha> ((i, r)#D) \<beta>"}, then there must exist a $\gamma$ such that @{term "Derives1 cfg \<alpha> i r \<gamma>"} and
-@{term "Derivation cfg \<gamma> D \<beta>"}. Obua then proves that both notions of a derivation are equivalent (lemma @{term derives_equiv_Derivation})
+@{term "Derivation \<G> \<alpha> ((i, r)#D) \<beta>"}, then there must exist a $\gamma$ such that @{term "Derives1 \<G> \<alpha> i r \<gamma>"} and
+@{term "Derivation \<G> \<gamma> D \<beta>"}. Note that we introduce a more convenient notation: e.g. @{term "Derivation \<alpha> D \<beta>"} is written  (@{term \<G>} $\vdash \alpha \Rightarrow^{\mathit{D}} \beta$). Obua then proves that both notions of a derivation are equivalent (lemma @{term derives_equiv_Derivation})
 \<close>
 
 type_synonym 'a derivation = "(nat \<times> 'a rule) list"
 
+(*<*)
+syntax
+  "Derivation" :: "'a cfg \<Rightarrow> 'a sentential \<Rightarrow> 'a derivation \<Rightarrow> 'a sentential \<Rightarrow> bool" ("_ \<turnstile> _ \<Rightarrow>\<^sup>_ _" [1000,0] 1000)
+(*>*)
+
 fun Derivation :: "'a cfg \<Rightarrow> 'a sentential \<Rightarrow> 'a derivation \<Rightarrow> 'a sentential \<Rightarrow> bool" where
   "Derivation _ \<alpha> [] \<beta> = (\<alpha> = \<beta>)"
-| "Derivation cfg \<alpha> (d#D) \<beta> = (\<exists>\<gamma>. Derives1 cfg \<alpha> (fst d) (snd d) \<gamma> \<and> Derivation cfg \<gamma> D \<beta>)"
+| "Derivation \<G> \<alpha> (d#D) \<beta> = (\<exists>\<gamma>. Derives1 \<G> \<alpha> (fst d) (snd d) \<gamma> \<and> Derivation \<G> \<gamma> D \<beta>)"
+
+(*<*)
+(*
+notation
+  Derives1 ("_ \<turnstile> _ \<^latex>\<open>\\ensuremath{\\xRightarrow{\<close>(_, _) \<^latex>\<open>}}\<close> _" [1000,0] 1000)
+
+notation
+  Derivation ("_ \<turnstile> _ \<^latex>\<open>\\ensuremath{\\xRightarrow{\<close>_ \<^latex>\<open>}}\<close> _" [1000,0] 1000)
+*)
+(*>*)
 
 lemma derives_equiv_Derivation:
-  shows "derives cfg \<alpha> \<beta> \<equiv> \<exists> D. Derivation cfg \<alpha> D \<beta>"
+  shows "\<G> \<turnstile> \<alpha> \<Rightarrow>\<^sup>* \<beta> \<equiv> \<exists>D. \<G> \<turnstile> \<alpha> \<Rightarrow>\<^sup>D \<beta>"
 (*<*)
   sorry
 (*>*)
@@ -476,9 +514,9 @@ definition of derivations defined above without explicit proof.
 \<close>
 
 lemma Derivation_append_rewrite:
-  assumes "Derivation cfg \<alpha> D (\<beta> @ \<gamma> @ \<delta>) "
-  assumes "Derivation cfg \<gamma> E \<gamma>'"
-  shows "\<exists>F. Derivation cfg \<alpha> F (\<beta> @ \<gamma>' @ \<delta>)"
+  assumes "\<G> \<turnstile> \<alpha> \<Rightarrow>\<^sup>D (\<beta> @ \<gamma> @ \<delta>) "
+  assumes "\<G> \<turnstile> \<gamma> \<Rightarrow>\<^sup>E \<gamma>'"
+  shows "\<exists>F. \<G> \<turnstile> \<alpha> \<Rightarrow>\<^sup>F (\<beta> @ \<gamma>' @ \<delta>)"
 (*<*)
   sorry
 (*>*)
@@ -488,9 +526,9 @@ And finally, we proof soundness of the @{term Complete} operation:
 \<close>
 
 lemma sound_Complete:
-  assumes wf: "wf_items cfg \<omega> I"
-  assumes sound: "sound_items cfg \<omega> I"
-  shows "sound_items cfg \<omega> (Complete k I)"
+  assumes wf: "wf_items \<G> \<omega> I"
+  assumes sound: "sound_items \<G> \<omega> I"
+  shows "sound_items \<G> \<omega> (Complete k I)"
 (*<*)
   sorry
 (*>*)
@@ -505,36 +543,36 @@ Let $z$ denote an arbitrary but fixed item of @{term "Complete k I"}. By the def
 
 Since $y$ is in bin $k$, it is complete and the set $I$ is sound (assumption \textit{sound}),
 there exists a derivation $E$ such that 
-  $$@{term "Derivation cfg [item_rule_head y] E (slice (item_origin y) (item_end y) \<omega>)"}$$
+  $$@{term "\<G> \<turnstile> [item_rule_head y] \<Rightarrow>\<^sup>E \<omega>[item_origin y..item_end y\<rangle>"}$$
 by lemma @{thm[source] derives_equiv_Derivation}. Similarly, since $x$ is in bin @{term "item_origin y"} and due to assumption \textit{sound},
 there exists a derivation $D$ such that
-  $$ @{term "Derivation cfg [item_rule_head x] D (slice (item_origin x) (item_origin y) \<omega> @ item_\<beta> x)"}$$
+  $$ @{term "\<G> \<turnstile> [item_rule_head x] \<Rightarrow>\<^sup>D \<omega>[item_origin x..item_origin y\<rangle> @ item_\<beta> x"}$$
 Note that @{term "item_\<beta> x = (item_rule_head y) # tl (item_\<beta> x)"} since the next symbol of $x$ is equal to
 the item rule head of $y$. Thus, by lemma @{thm[source] Derivation_append_rewrite}, and the definition of $D$ and $E$,
 there exists a derivation $F$ such that
 
 \begin{equation*}
 \begin{split}
-  & @{term "Derivation cfg [item_rule_head x] F (slice (item_origin x) (item_origin y) \<omega>)"} \, @ \\
-  & \quad \quad @{term "slice (item_origin y) (item_end y) \<omega> @ tl (item_\<beta> x)"}
+  & @{term "\<G> \<turnstile> [item_rule_head x] \<Rightarrow>\<^sup>F \<omega>[item_origin x..item_origin y\<rangle>"} \, @ \\
+  & \quad \quad @{term "\<omega>[item_origin y..item_end y\<rangle> @ tl (item_\<beta> x)"}
 \end{split}
 \end{equation*}
 
 Additionally, we know that $x$ and $y$ are well-formed items due to the facts that $x$ is in bin @{term "item_origin y"},
-$y$ is in bin $k$, and the assumption @{term "wf_items cfg \<omega> I"}. Thus, we can discharge the assumptions of
+$y$ is in bin $k$, and the assumption @{term "wf_items \<G> \<omega> I"}. Thus, we can discharge the assumptions of
 lemma @{thm[source] slice_append} (@{term "item_origin x \<le> item_origin y"} and @{term "item_origin y \<le> item_end y"})
 and have 
-  $$@{term "Derivation cfg [item_rule_head x] F (slice (item_origin x) (item_end y) \<omega> @ tl (item_\<beta> x))"}$$
+  $$@{term "\<G> \<turnstile> [item_rule_head x] \<Rightarrow>\<^sup>F \<omega>[item_origin x..item_end y\<rangle> @ tl (item_\<beta> x)"}$$
 
 Moreover, since @{term "z = inc_item x k"} and the next symbol of x is the item rule head of y, it follows
-that @{term "tl (item_\<beta> x) = item_\<beta> z"}, and ultimately @{term "sound_item cfg \<omega> z"}, again by the definition
+that @{term "tl (item_\<beta> x) = item_\<beta> z"}, and ultimately @{term "sound_item \<G> \<omega> z"}, again by the definition
 of $z$ and lemma @{thm[source] derives_equiv_Derivation}.
 
 \end{proof}
 \<close>
 
 lemma sound_Init:
-  shows "sound_items cfg \<omega> (Init cfg)"
+  shows "sound_items \<G> \<omega> (Init \<G>)"
 (*<*)
   sorry
 (*>*)
@@ -542,9 +580,9 @@ lemma sound_Init:
 text\<open>\<close>
 
 lemma sound_Scan:
-  assumes "wf_items cfg \<omega> I"
-  assumes "sound_items cfg \<omega> I"
-  shows "sound_items cfg \<omega> (Scan k \<omega> I)"
+  assumes "wf_items \<G> \<omega> I"
+  assumes "sound_items \<G> \<omega> I"
+  shows "sound_items \<G> \<omega> (Scan k \<omega> I)"
 (*<*)
   sorry
 (*>*)
@@ -552,8 +590,8 @@ lemma sound_Scan:
 text\<open>\<close>
 
 lemma sound_Predict:
-  assumes "sound_items cfg \<omega> I"
-  shows "sound_items cfg \<omega> (Predict k cfg I)"
+  assumes "sound_items \<G> \<omega> I"
+  shows "sound_items \<G> \<omega> (Predict k \<G> I)"
 (*<*)
   sorry
 (*>*)
@@ -561,9 +599,9 @@ lemma sound_Predict:
 text\<open>\<close>
 
 lemma sound_Earley_step:
-  assumes "wf_items cfg \<omega> I"
-  assumes "sound_items cfg \<omega> I" 
-  shows "sound_items cfg \<omega> (Earley_step k cfg \<omega> I)"
+  assumes "wf_items \<G> \<omega> I"
+  assumes "sound_items \<G> \<omega> I" 
+  shows "sound_items \<G> \<omega> (Earley_step k \<G> \<omega> I)"
 (*<*)
   sorry
 (*>*)
@@ -571,9 +609,9 @@ lemma sound_Earley_step:
 text\<open>\<close>
 
 lemma sound_funpower:
-  assumes "wf_items cfg \<omega> I"
-  assumes "sound_items cfg \<omega> I"
-  shows "sound_items cfg \<omega> (funpower (Earley_step k cfg \<omega>) n I)"
+  assumes "wf_items \<G> \<omega> I"
+  assumes "sound_items \<G> \<omega> I"
+  shows "sound_items \<G> \<omega> (funpower (Earley_step k \<G> \<omega>) n I)"
 (*<*)
   sorry
 (*>*)
@@ -581,9 +619,9 @@ lemma sound_funpower:
 text\<open>\<close>
 
 lemma sound_Earley_bin:
-  assumes "wf_items cfg \<omega> I"
-  assumes "sound_items cfg \<omega> I"
-  shows "sound_items cfg \<omega> (Earley_bin k cfg \<omega> I)"
+  assumes "wf_items \<G> \<omega> I"
+  assumes "sound_items \<G> \<omega> I"
+  shows "sound_items \<G> \<omega> (Earley_bin k \<G> \<omega> I)"
 (*<*)
   sorry
 (*>*)
@@ -591,7 +629,7 @@ lemma sound_Earley_bin:
 text\<open>\<close>
 
 lemma sound_Earley_bin0:
-  shows "sound_items cfg \<omega> (Earley_bin 0 cfg \<omega> (Init cfg))"
+  shows "sound_items \<G> \<omega> (Earley_bin 0 \<G> \<omega> (Init \<G>))"
 (*<*)
   sorry
 (*>*)
@@ -599,7 +637,7 @@ lemma sound_Earley_bin0:
 text\<open>\<close>
 
 lemma sound_Earley:
-  shows "sound_items cfg \<omega> (Earley k cfg \<omega>)"
+  shows "sound_items \<G> \<omega> (Earley k \<G> \<omega>)"
 (*<*)
   sorry
 (*>*)
@@ -607,7 +645,7 @@ lemma sound_Earley:
 text\<open>\<close>
 
 lemma sound_\<E>arley:
-  shows "sound_items cfg \<omega> (\<E>arley cfg \<omega>)"
+  shows "sound_items \<G> \<omega> (\<E>arley \<G> \<omega>)"
 (*<*)
   sorry
 (*>*)
@@ -620,8 +658,8 @@ of the input $\omega$ from the start symbol of the grammar.
 \<close>
 
 theorem soundness:
-  assumes "recognizing (\<E>arley cfg \<omega>) cfg \<omega>"
-  shows "derives cfg [\<SS> cfg] \<omega>"
+  assumes "recognizing (\<E>arley \<G> \<omega>) \<G> \<omega>"
+  shows "\<G> \<turnstile> [\<SS> \<G>] \<Rightarrow>\<^sup>* \<omega>"
 (*<*)
   sorry
 (*>*)
@@ -636,7 +674,7 @@ and soundness proofs presented previously. We directly start to prove three prop
 function that correspond conceptually to the three different operations that can occur while generating
 the bins.
 
-We need three simple lemmas concerning the @{term Earley_bin} function, stated without explicit proof: (1) @{term "Earley_bin k cfg \<omega> I"}
+We need three simple lemmas concerning the @{term Earley_bin} function, stated without explicit proof: (1) @{term "Earley_bin k \<G> \<omega> I"}
 only (potentially) changes bins $k$ and $k+1$ (lemma @{term Earley_bin_bin_idem}); (2) the @{term Earley_step}
 operation is subsumed by the @{term Earley_bin} operation, since it computes the limit of @{term Earley_step}
 (lemma @{term Earley_step_sub_Earley_bin}); and (3) the function @{term Earley_bin} is idempotent (lemma @{term Earley_bin_idem}).
@@ -645,7 +683,7 @@ operation is subsumed by the @{term Earley_bin} operation, since it computes the
 lemma Earley_bin_bin_idem:
   assumes "i \<noteq> k"
   assumes "i \<noteq> k+1" 
-  shows "bin (Earley_bin k cfg \<omega> I) i = bin I i"
+  shows "bin (Earley_bin k \<G> \<omega> I) i = bin I i"
 (*<*)
   sorry
 (*>*)
@@ -653,7 +691,7 @@ lemma Earley_bin_bin_idem:
 text\<open>\<close>
 
 lemma Earley_step_sub_Earley_bin:
-  shows "Earley_step k cfg \<omega> I \<subseteq> Earley_bin k cfg inp I"
+  shows "Earley_step k \<G> \<omega> I \<subseteq> Earley_bin k \<G> \<omega> I"
 (*<*)
   sorry
 (*>*)
@@ -661,7 +699,7 @@ lemma Earley_step_sub_Earley_bin:
 text\<open>\<close>
 
 lemma Earley_bin_idem:
-  shows "Earley_bin k cfg \<omega> (Earley_bin k cfg \<omega> I) = Earley_bin k cfg \<omega> I"
+  shows "Earley_bin k \<G> \<omega> (Earley_bin k \<G> \<omega> I) = Earley_bin k \<G> \<omega> I"
 (*<*)
   sorry
 (*>*)
@@ -672,11 +710,11 @@ text\<open>Next, we proof lemma @{term Scan_Earley} in detail: it describes unde
 
 lemma Scan_Earley:
   assumes "i+1 \<le> k"
-  assumes "x \<in> bin (Earley k cfg \<omega>) i"
+  assumes "x \<in> bin (Earley k \<G> \<omega>) i"
   assumes "next_symbol x = Some a"
-  assumes "k \<le> length \<omega>"
+  assumes "k \<le> |\<omega>|"
   assumes "\<omega>!i = a"
-  shows "inc_item x (i+1) \<in> Earley k cfg \<omega>"
+  shows "inc_item x (i+1) \<in> Earley k \<G> \<omega>"
 (*<*)
   sorry
 (*>*)
@@ -688,25 +726,25 @@ The proof is by induction in $k$ for arbitrary $i$, $x$, and $a$:
 
 The base case @{term "k = (0::nat)"} is trivial, since we have the assumption @{term "i+(1::nat) \<le> 0"}.
 
-For the induction step we can assume @{term "i+(1::nat) \<le> k+1"}, @{term "k+(1::nat) \<le> length \<omega>"},
-@{term "x \<in> bin (Earley (k+1) cfg \<omega>) i"} , @{term "next_symbol x = Some a"}, and @{term "\<omega>!i = a"}.
-Assumptions @{term "x \<in> bin (Earley (k+1) cfg \<omega>) i"} and @{term "i+(1::nat) \<le> k+1"} imply that
-@{term "x \<in> bin (Earley k cfg inp) i"} by lemma @{thm[source] Earley_bin_bin_idem}.
+For the induction step we can assume @{term "i+(1::nat) \<le> k+1"}, @{term "k+(1::nat) \<le> |\<omega>|"},
+@{term "x \<in> bin (Earley (k+1) \<G> \<omega>) i"} , @{term "next_symbol x = Some a"}, and @{term "\<omega>!i = a"}.
+Assumptions @{term "x \<in> bin (Earley (k+1) \<G> \<omega>) i"} and @{term "i+(1::nat) \<le> k+1"} imply that
+@{term "x \<in> bin (Earley k \<G> \<omega>) i"} by lemma @{thm[source] Earley_bin_bin_idem}.
 
 We then consider two cases: 
 \begin{itemize}
   \item @{term "i+(1::nat) \<le> k"}: We can apply the induction hypothesis using assumptions
-    @{term "k+(1::nat) \<le> length \<omega>"}, @{term "next_symbol x = Some a"}, @{term "\<omega>!i = a"} and 
-    additionally @{term "x \<in> bin (Earley k cfg inp) i"} and have @{term "inc_item x (i+1) \<in> Earley k cfg \<omega>"}.
+    @{term "k+(1::nat) \<le> |\<omega>|"}, @{term "next_symbol x = Some a"}, @{term "\<omega>!i = a"} and 
+    additionally @{term "x \<in> bin (Earley k \<G> \<omega>) i"} and have @{term "inc_item x (i+1) \<in> Earley k \<G> \<omega>"}.
     The statement to proof follows by lemma @{thm[source] Earley_step_sub_Earley_bin} and the definition of
     @{term Earley_step}.
   \item @{term "i+(1::nat) > k"}: We have @{term "i = k"}, since @{term "i+(1::nat) \<le> k+1"}.
-    Thus, we have @{term "inc_item x (i+1) \<in> Scan k \<omega> (Earley k cfg \<omega>)"} using assumptions
-    @{term "k+(1::nat) \<le> length \<omega>"}, @{term "next_symbol x = Some a"}, @{term "\<omega>!i = a"}, and additionally
-    @{term "x \<in> bin (Earley k cfg inp) i"} by the definition of the @{term Scan} operation.
-    This in turn implies @{term "inc_item x (i+1) \<in> Earley_step k cfg \<omega> (Earley k cfg \<omega>)"} by lemma @{thm[source] Earley_step_sub_Earley_bin}
+    Thus, we have @{term "inc_item x (i+1) \<in> Scan k \<omega> (Earley k \<G> \<omega>)"} using assumptions
+    @{term "k+(1::nat) \<le> |\<omega>|"}, @{term "next_symbol x = Some a"}, @{term "\<omega>!i = a"}, and additionally
+    @{term "x \<in> bin (Earley k \<G> \<omega>) i"} by the definition of the @{term Scan} operation.
+    This in turn implies @{term "inc_item x (i+1) \<in> Earley_step k \<G> \<omega> (Earley k \<G> \<omega>)"} by lemma @{thm[source] Earley_step_sub_Earley_bin}
     and the definition of @{term Earley_step}. Since the function @{term Earley_bin} is idempotent
-    (lemma @{thm[source] Earley_bin_idem}), we have @{term "inc_item x (i+1) \<in> Earley k cfg \<omega>"} by definition of
+    (lemma @{thm[source] Earley_bin_idem}), we have @{term "inc_item x (i+1) \<in> Earley k \<G> \<omega>"} by definition of
     @{term Earley}. And again, the final statement follows by lemma @{thm[source] Earley_step_sub_Earley_bin} and the definition of
     @{term Earley_step}.
 \end{itemize}
@@ -716,10 +754,10 @@ We then consider two cases:
 
 lemma Predict_Earley:
   assumes "i \<le> k"
-  assumes "x \<in> bin (Earley k cfg \<omega>) i"
+  assumes "x \<in> bin (Earley k \<G> \<omega>) i"
   assumes "next_symbol x = Some N"
-  assumes "(N,\<alpha>) \<in> set (\<RR> cfg)"
-  shows "init_item (N,\<alpha>) i \<in> Earley k cfg \<omega>"
+  assumes "(N,\<alpha>) \<in> set (\<RR> \<G>)"
+  shows "init_item (N,\<alpha>) i \<in> Earley k \<G> \<omega>"
 (*<*)
   sorry
 (*>*)
@@ -729,14 +767,14 @@ text\<open>\<close>
 lemma Complete_Earley:
   assumes "i \<le> j"
   assumes "j \<le> k"
-  assumes "x \<in> bin (Earley k cfg \<omega>) i"
+  assumes "x \<in> bin (Earley k \<G> \<omega>) i"
   assumes "next_symbol x = Some N"
-  assumes "(N,\<alpha>) \<in> set (\<RR> cfg)"
-  assumes "y \<in> bin (Earley k cfg \<omega>) j"
+  assumes "(N,\<alpha>) \<in> set (\<RR> \<G>)"
+  assumes "y \<in> bin (Earley k \<G> \<omega>) j"
   assumes "item_rule y = (N,\<alpha>)"
   assumes "i = item_origin y"
   assumes "is_complete y"
-  shows "inc_item x j \<in> Earley k cfg \<omega>"
+  shows "inc_item x j \<in> Earley k \<G> \<omega>"
 (*<*)
   sorry
 (*>*)
@@ -774,16 +812,16 @@ Lemma @{term partially_completed_upto} then formalizes the core idea: if
 $N \rightarrow \, \alpha \bullet \beta, i, j$ in a set of items $I$ and there exists a derivation
 $\beta \xRightarrow{D} \omega[j..k)$, then $I$ also contains the complete item 
 $N \rightarrow \, \alpha \beta \bullet, i, k$. Note that this
-holds only if @{term "j \<le> k"}, @{term "k \<le> length \<omega>"}, all items of $I$ are well-formed and most importantly
+holds only if @{term "j \<le> k"}, @{term "k \<le> |\<omega>|"}, all items of $I$ are well-formed and most importantly
 $I$ must be @{term partially_completed} up to the length of the derivation $D$.
 \<close>
 
 definition partially_completed :: "nat \<Rightarrow> 'a cfg \<Rightarrow> 'a sentential \<Rightarrow> 'a items \<Rightarrow> ('a derivation \<Rightarrow> bool) \<Rightarrow> bool" where
-  "partially_completed k cfg \<omega> I P \<equiv>
+  "partially_completed k \<G> \<omega> I P \<equiv>
     \<forall>i j x a D.
-      i \<le> j \<and> j \<le> k \<and> k \<le> length \<omega> \<and>
+      i \<le> j \<and> j \<le> k \<and> k \<le> |\<omega>| \<and>
       x \<in> bin I i \<and> next_symbol x = Some a \<and>
-      Derivation cfg [a] D (slice i j \<omega>) \<and> P D \<longrightarrow>
+      \<G> \<turnstile> [a] \<Rightarrow>\<^sup>D \<omega>[i..j\<rangle> \<and> P D \<longrightarrow>
       inc_item x j \<in> I"
 
 text\<open>
@@ -800,9 +838,8 @@ move on to the proof of lemmas @{term partially_completed_upto} and @{term parti
 \<close>
 
 lemma Derivation_append_split:
-  assumes "Derivation cfg (\<alpha>@\<beta>) D \<gamma>"
-  shows "\<exists>E F \<alpha>' \<beta>'. Derivation cfg \<alpha> E \<alpha>' \<and> Derivation cfg \<beta> F \<beta>' \<and> \<gamma> = \<alpha>' @ \<beta>' \<and>
-    length E \<le> length D \<and> length F \<le> length D"
+  assumes "\<G> \<turnstile> (\<alpha>@\<beta>) \<Rightarrow>\<^sup>D \<gamma>"
+  shows "\<exists>E F \<alpha>' \<beta>'. \<G> \<turnstile> \<alpha> \<Rightarrow>\<^sup>E \<alpha>' \<and> \<G> \<turnstile> \<beta> \<Rightarrow>\<^sup>F \<beta>' \<and> \<gamma> = \<alpha>' @ \<beta>' \<and> |E| \<le> |D| \<and> |F| \<le> |D|"
 (*<*)
   sorry
 (*>*)
@@ -811,8 +848,8 @@ text\<open>\<close>
 
 lemma slice_append_split:
   assumes "i \<le> k"
-  assumes "slice i k xs = ys @ zs"
-  shows "\<exists>j. ys = slice i j xs \<and> zs = slice j k xs \<and> i \<le> b \<and> b \<le> k"
+  assumes "xs[i..k\<rangle> = ys @ zs"
+  shows "\<exists>j. ys = xs[i..j\<rangle> \<and> zs = xs[j..k\<rangle> \<and> i \<le> b \<and> b \<le> k"
 (*<*)
   sorry
 (*>*)
@@ -820,14 +857,14 @@ lemma slice_append_split:
 text\<open>\<close>
 
 lemma partially_completed_upto:
-  assumes "wf_items cfg \<omega> I"
+  assumes "wf_items \<G> \<omega> I"
   assumes "j \<le> k" 
-  assumes "k \<le> length \<omega>"
+  assumes "k \<le> |\<omega>|"
   assumes "x = Item (N,\<alpha>) b i j"
   assumes "x \<in> I"
-  assumes "Derivation cfg (item_\<beta> x) D (slice j k \<omega>)"
-  assumes "partially_completed k cfg \<omega> I (\<lambda>D'. length D' \<le> length D)"
-  shows "Item (N,\<alpha>) (length \<alpha>) i k \<in> I"
+  assumes "\<G> \<turnstile> (item_\<beta> x) \<Rightarrow>\<^sup>D \<omega>[j..k\<rangle>"
+  assumes "partially_completed k \<G> \<omega> I (\<lambda>D'. |D'| \<le> |D| )"
+  shows "Item (N,\<alpha>) |\<alpha>| i k \<in> I"
 (*<*)
   sorry
 (*>*)
@@ -838,48 +875,48 @@ text\<open>
 The proof is by induction on (@{term "item_\<beta> x"}) for arbitrary $b$, $i$, $j$, $k$, $N$, $\alpha$,
 $x$, and $D$:
 
-For the base case we have @{term "item_\<beta> x = []"} and need to show that @{term "Item (N, \<alpha>) (length \<alpha>) i k \<in> I"}:
+For the base case we have @{term "item_\<beta> x = []"} and need to show that @{term "Item (N, \<alpha>) |\<alpha>| i k \<in> I"}:
 
 The bullet of $x$ is right before @{term "item_\<beta> x"}, or @{term "item_\<alpha> x = \<alpha>"}. Thus, the value of the
-bullet must be equal to the length of $\alpha$, which implies @{term "x = Item (N,\<alpha>) (length \<alpha>) i j"}, since $x$
+bullet must be equal to the length of $\alpha$, which implies @{term "x = Item (N,\<alpha>) |\<alpha>| i j"}, since $x$
 is a well-formed item and @{term "item_\<beta> x = []"}.
 
-We also know that $j = k$: we have @{term "Derivation cfg (item_\<beta> x) D (slice j k \<omega>)"} and
-@{term "item_\<beta> x = []"} which in turn implies that @{term "slice j k \<omega> = []"}, and thus $j = k$.
+We also know that $j = k$: we have @{term "\<G> \<turnstile> (item_\<beta> x) \<Rightarrow>\<^sup>D \<omega>[j..k\<rangle>"} and
+@{term "item_\<beta> x = []"} which in turn implies that @{term "\<omega>[j..k\<rangle> = []"}, and thus $j = k$.
 
-Hence, the statement follows from the assumption @{term "x \<in> I"} and the fact that @{term "x = Item (N,\<alpha>) (length \<alpha>) i j"}.
+Hence, the statement follows from the assumption @{term "x \<in> I"} and the fact that @{term "x = Item (N,\<alpha>) |\<alpha>| i j"}.
 
-For the induction step we have @{term "item_\<beta> x = a#as"} and need to show that @{term "Item (N, \<alpha>) (length \<alpha>) i k \<in> I"}:
+For the induction step we have @{term "item_\<beta> x = a#as"} and need to show that @{term "Item (N, \<alpha>) |\<alpha>| i k \<in> I"}:
 
 Using lemmas @{thm[source] Derivation_append_split} and @{thm[source] slice_append_split}
 there exists an index $j'$ and derivations $E$ and $F$ such that
 
 \begin{equation*}
 \begin{split}
- @{term "Derivation cfg [a] E (slice j j' \<omega>)"} & @{term "length E \<le> length D"} \\
- @{term "Derivation cfg as F (slice j' k \<omega>)"} & @{term "length F \<le> length D"} \\
+ @{term "\<G> \<turnstile> [a] \<Rightarrow>\<^sup>E \<omega>[j..j'\<rangle>"} \qquad & @{term "|E| \<le> |D|"} \\
+ @{term "\<G> \<turnstile> as \<Rightarrow>\<^sup>F \<omega>[j'..k\<rangle>"} \qquad & @{term "|F| \<le> |D|"} \\
  @{term "j \<le> j'"} \qquad @{term "j' \<le> k"} &
 \end{split}
 \end{equation*}
 
 Using the facts about derivation $E$, @{term "j \<le> j'"}, @{term "j' \<le> k"} and the assumptions
-@{term "k \<le> length \<omega>"}, @{term "x = Item (N, \<alpha>) b i j"}, @{term "x \<in> I"}, @{term "next_symbol x = Some a"}
+@{term "k \<le> |\<omega>|"}, @{term "x = Item (N, \<alpha>) b i j"}, @{term "x \<in> I"}, @{term "next_symbol x = Some a"}
 (since @{term "item_\<beta> x = a#as"}) and @{term "x \<in> bin I j"}, we have @{term "inc_item x j' \<in> I"} by the
-assumption @{term "partially_completed k cfg \<omega> I (\<lambda>D'. length D' \<le> length D)"}.
+assumption @{term "partially_completed k \<G> \<omega> I (\<lambda>D'. |D'| \<le> |D| )"}.
 Note that @{term "inc_item x j' = Item (N, \<alpha>) (b+1) i j'"}, which we will from now on refer to as item $x'$.
 
-From @{term "partially_completed k cfg \<omega> I (\<lambda>D'. length D' \<le> length D)"} and @{term "length F \<le> length D"}
-follows @{term "partially_completed k cfg \<omega> I (\<lambda>D'. length D' \<le> length F)"}. We also have @{term "as = item_\<beta> x'"}
+From @{term "partially_completed k \<G> \<omega> I (\<lambda>D'. |D'| \<le> |D| )"} and @{term "|F| \<le> |D|"}
+follows @{term "partially_completed k \<G> \<omega> I (\<lambda>D'. |D'| \<le> |F| )"}. We also have @{term "as = item_\<beta> x'"}
 and @{term "x' \<in> I"}. Hence, we can apply the induction hypothesis for $x'$ using additionally the assumptions
-@{term "wf_items cfg \<omega> I"}, @{term "k \<le> length \<omega>"}, and the facts about derivation $F$ from above, and
-have @{term "Item (N, \<alpha>) (length \<alpha>) i k \<in> I"}, what we intended to show.
+@{term "wf_items \<G> \<omega> I"}, @{term "k \<le> |\<omega>|"}, and the facts about derivation $F$ from above, and
+have @{term "Item (N, \<alpha>) |\<alpha>| i k \<in> I"}, what we intended to show.
 
 \end{proof}
 \<close>
 
 lemma partially_completed_Earley:
-  assumes "wf_cfg cfg"
-  shows "partially_completed k cfg \<omega> (Earley k cfg \<omega>) (\<lambda>_. True)"
+  assumes "wf_\<G> \<G>"
+  shows "partially_completed k \<G> \<omega> (Earley k \<G> \<omega>) (\<lambda>_. True)"
 (*<*)
   sorry
 (*>*)
@@ -890,46 +927,46 @@ text\<open>
 Let $x$, $i$, $a$, $D$, and $j$ be arbitrary but fixed.
 
 By definition of @{term partially_completed} we can assume @{term "i \<le> j"}, @{term "j \<le> k"},
-@{term "k \<le> length \<omega>"}, @{term "x \<in> bin (Earley k cfg \<omega>) i"}, @{term "next_symbol x = Some a"},
-@{term "Derivation cfg [a] D (slice i j \<omega>)"}, and need to show @{term "inc_item x j \<in> Earley k cfg \<omega>"}.
+@{term "k \<le> |\<omega>|"}, @{term "x \<in> bin (Earley k \<G> \<omega>) i"}, @{term "next_symbol x = Some a"},
+@{term "\<G> \<turnstile> [a] \<Rightarrow>\<^sup>D \<omega>[i..j\<rangle>"}, and need to show @{term "inc_item x j \<in> Earley k \<G> \<omega>"}.
 
-We proof this by complete induction on @{term "length D"} for arbitrary $x$, $i$, $a$, $j$, and $D$,
+We proof this by complete induction on @{term "|D|"} for arbitrary $x$, $i$, $a$, $j$, and $D$,
 and split the proof into two different cases:
 
 \begin{itemize}
 
-  \item @{term "D = []"}: Since @{term "Derivation cfg [a] D (slice i j \<omega>)"}, we have @{term "[a] = slice i j \<omega>"},
+  \item @{term "D = []"}: Since @{term "\<G> \<turnstile> [a] \<Rightarrow>\<^sup>D \<omega>[i..j\<rangle>"}, we have @{term "[a] = \<omega>[i..j\<rangle>"},
   and consequently @{term "\<omega>!i = a"} and @{term "j = i+(1::nat)"}. Now we discharge the assumptions of lemma @{thm[source] Scan_Earley},
-  using additionally @{term "x \<in> bin (Earley k cfg \<omega>) i"}, @{term "next_symbol x = Some a"}, and @{term "j \<le> length \<omega>"},
-  and have @{term "inc_item x (i+1) \<in> Earley k cfg \<omega>"} which finishes the proof since @{term "j = i+(1::nat)"}.
+  using additionally @{term "x \<in> bin (Earley k \<G> \<omega>) i"}, @{term "next_symbol x = Some a"}, and @{term "j \<le> |\<omega>|"},
+  and have @{term "inc_item x (i+1) \<in> Earley k \<G> \<omega>"} which finishes the proof since @{term "j = i+(1::nat)"}.
   
-  \item @{term "D = d#D'"}: Since @{term "Derivation cfg [a] D (slice i j \<omega>)"}, there exists an $\alpha$ such that
-  @{term "Derives1 cfg [a] (fst d) (snd d) \<alpha>"} and @{term "Derivation cfg \<alpha> D' (slice i j \<omega>)"}. From the definition
+  \item @{term "D = d#\<D>"}: Since @{term "\<G> \<turnstile> [a] \<Rightarrow>\<^sup>D \<omega>[i..j\<rangle>"}, there exists an $\alpha$ such that
+  @{term "Derives1 \<G> [a] (fst d) (snd d) \<alpha>"} and @{term "\<G> \<turnstile> \<alpha> \<Rightarrow>\<^sup>\<D> \<omega>[i..j\<rangle>"}. From the definition
   of @{term "Derives1"} we see that there exists a non-terminal $N$ such that @{term "a = N"},
-  @{term "(N, \<alpha>) \<in> set (\<RR> cfg)"}, @{term "fst d = (0::nat)"}, and @{term "snd d = (N, \<alpha>)"}.
+  @{term "(N, \<alpha>) \<in> set (\<RR> \<G>)"}, @{term "fst d = (0::nat)"}, and @{term "snd d = (N, \<alpha>)"}.
 
-  Let $y$ denote @{term "Item (N,\<alpha>) 0 i i"}. Since we have @{term "i \<le> k"}, @{term "x \<in> bin (Earley k cfg \<omega>) i"},
-  and @{term "next_symbol x = Some a"} by assumption, we showed that @{term "a = N"} and @{term "(N, \<alpha>) \<in> set (\<RR> cfg)"},
-  and $y$ is an initial item, we have @{term "y \<in> Earley k cfg \<omega>"} by lemma @{thm[source] Predict_Earley}.
+  Let $y$ denote @{term "Item (N,\<alpha>) 0 i i"}. Since we have @{term "i \<le> k"}, @{term "x \<in> bin (Earley k \<G> \<omega>) i"},
+  and @{term "next_symbol x = Some a"} by assumption, we showed that @{term "a = N"} and @{term "(N, \<alpha>) \<in> set (\<RR> \<G>)"},
+  and $y$ is an initial item, we have @{term "y \<in> Earley k \<G> \<omega>"} by lemma @{thm[source] Predict_Earley}.
 
   Next, we use lemma @{thm[source] partially_completed_upto} to show that we the completed version
-  of item $y$ is also present in the $j$-th bin of @{term "Earley k cfg \<omega>"} since we have a derivation
-  $\alpha \xRightarrow{D'} \, \omega[i..j)$, or @{term "Item (N,\<alpha>) (length \<alpha>) i j \<in> bin (Earley k cfg \<omega>) j"}:
-  we have @{term "i \<le> j"}, @{term "j \<le> length \<omega>"} by assumption; have proven @{term "y \<in> Earley k cfg \<omega>"};
-  and have @{term "wf_items cfg \<omega> (Earley k cfg \<omega>)"} by lemma @{thm[source] wf_Earley}. Additionally, we know
-  @{term "Derivation cfg (item_\<beta> y) D' (slice i j \<omega>)"} since @{term "Derivation cfg [a] D' (slice i j \<omega>)"} and
+  of item $y$ is also present in the $j$-th bin of @{term "Earley k \<G> \<omega>"} since we have a derivation
+  @{term "\<G> \<turnstile> \<alpha> \<Rightarrow>\<^sup>\<D> \<omega>[i..j\<rangle>"}, or @{term "Item (N,\<alpha>) |\<alpha>| i j \<in> bin (Earley k \<G> \<omega>) j"}:
+  we have @{term "i \<le> j"}, @{term "j \<le> |\<omega>|"} by assumption; have proven @{term "y \<in> Earley k \<G> \<omega>"};
+  and have @{term "wf_items \<G> \<omega> (Earley k \<G> \<omega>)"} by lemma @{thm[source] wf_Earley}. Additionally, we know
+  @{term "\<G> \<turnstile> (item_\<beta> y) \<Rightarrow>\<^sup>\<D> \<omega>[i..j\<rangle>"} since @{term "\<G> \<turnstile> [a] \<Rightarrow>\<^sup>\<D> \<omega>[i..j\<rangle>"} and
   @{term "a = N"}, by the definition of item $y$. Finally, we use the induction hypothesis to show
-  @{term "partially_completed k cfg \<omega> (Earley k cfg \<omega>) (\<lambda>E. length E \<le> length D')"}, since @{term "length D' \<le> length D"}
+  @{term "partially_completed k \<G> \<omega> (Earley k \<G> \<omega>) (\<lambda>E. |E| \<le> |\<D>| )"}, since @{term "|\<D>| \<le> |D|"}
   by definition of @{term partially_completed}, using once again all of our assumptions. This in turn implies
-  @{term "partially_completed j cfg \<omega> (Earley k cfg \<omega>) (\<lambda>E. length E \<le> length D')"} since
+  @{term "partially_completed j \<G> \<omega> (Earley k \<G> \<omega>) (\<lambda>E. |E| \<le> |\<D>| )"} since
   @{term "j \<le> k"} by definition of @{term partially_completed}. Now we can use lemma @{thm[source] partially_completed_upto}, and the statement follows
   from the definition of a bin.
 
-  Finally, we prove @{term "inc_item x j \<in> Earley k cfg \<omega>"} by lemma @{thm[source] Complete_Earley}:
-  once again we have @{term "i \<le> j"}, @{term "j \<le> k"}, and @{term "x \<in> bin (Earley k cfg \<omega>) i"} by assumption.
+  Finally, we prove @{term "inc_item x j \<in> Earley k \<G> \<omega>"} by lemma @{thm[source] Complete_Earley}:
+  once again we have @{term "i \<le> j"}, @{term "j \<le> k"}, and @{term "x \<in> bin (Earley k \<G> \<omega>) i"} by assumption.
   We also know that @{term "next_symbol x = Some N"}, due to our assumption @{term "next_symbol x = Some a"}
-  and @{term "a = N"}. Moreover, we have @{term "(N, \<alpha>) \<in> set (\<RR> cfg)"} and most importantly
-  @{term "Item (N,\<alpha>) (length \<alpha>) i j \<in> bin (Earley k cfg \<omega>) j"}, which concludes this proof.
+  and @{term "a = N"}. Moreover, we have @{term "(N, \<alpha>) \<in> set (\<RR> \<G>)"} and most importantly
+  @{term "Item (N,\<alpha>) |\<alpha>| i j \<in> bin (Earley k \<G> \<omega>) j"}, which concludes this proof.
   
 \end{itemize}
 
@@ -942,8 +979,8 @@ by definition of @{term \<E>arley}.
 \<close>
 
 lemma partially_completed_\<E>arley:
-  assumes "wf_cfg cfg"
-  shows "partially_completed (length \<omega>) cfg \<omega> (\<E>arley cfg \<omega>) (\<lambda>_. True)"
+  assumes "wf_\<G> \<G>"
+  shows "partially_completed |\<omega>| \<G> \<omega> (\<E>arley \<G> \<omega>) (\<lambda>_. True)"
 (*<*)
   sorry
 (*>*)
@@ -952,10 +989,10 @@ text\<open>And finally, we can proof completeness of Earley's algorithm, obtaini
 due to lemma @{thm[source] soundness}.\<close>
 
 theorem completeness:
-  assumes "wf_cfg cfg"
-  assumes "is_sentence cfg \<omega>"
-  assumes "derives cfg [\<SS> cfg] \<omega>"
-  shows "recognizing (\<E>arley cfg \<omega>) cfg \<omega>"
+  assumes "wf_\<G> \<G>"
+  assumes "is_sentence \<G> \<omega>"
+  assumes "\<G> \<turnstile> [\<SS> \<G>] \<Rightarrow>\<^sup>* \<omega>"
+  shows "recognizing (\<E>arley \<G> \<omega>) \<G> \<omega>"
 (*<*)
   sorry
 (*>*)
@@ -963,22 +1000,22 @@ theorem completeness:
 text\<open>
 \begin{proof}
 
-We know that there exists an $\alpha$ and a derivation $D$ such that @{term "(\<SS> cfg, \<alpha>) \<in> set (\<RR> cfg)"} and @{term "Derivation cfg \<alpha> D \<omega>"},
-since @{term "derives cfg [\<SS> cfg] \<omega>"}. Let $x$ denote the item @{term "Item (\<SS> cfg, \<alpha>) 0 0 0"}. By definition
-of $x$ and the @{term Init} operation and @{term \<E>arley} function, and the fact that @{term "Init cfg \<subseteq> Earley k cfg \<omega>"}, 
-we have @{term "x \<in> \<E>arley cfg \<omega>"}, moreover we have @{term "partially_completed (length \<omega>) cfg \<omega> (\<E>arley cfg \<omega>) (\<lambda>_. True)"}
-using lemma @{thm[source] partially_completed_\<E>arley} and assumption @{term "wf_cfg cfg"}, and thus have
-@{term "Item (\<SS> cfg,\<alpha>) (length \<alpha>) 0 (length \<omega>) \<in> \<E>arley cfg \<omega>"} by lemmas @{thm[source] partially_completed_upto} and
-@{thm[source] wf_\<E>arley} and the definition of @{term partially_completed}. The statement @{term "recognizing (\<E>arley cfg \<omega>) cfg \<omega>"}
+We know that there exists an $\alpha$ and a derivation $D$ such that @{term "(\<SS> \<G>, \<alpha>) \<in> set (\<RR> \<G>)"} and @{term "\<G> \<turnstile> \<alpha> \<Rightarrow>\<^sup>D \<omega>"},
+since @{term "\<G> \<turnstile> [\<SS> \<G>] \<Rightarrow>\<^sup>* \<omega>"}. Let $x$ denote the item @{term "Item (\<SS> \<G>, \<alpha>) 0 0 0"}. By definition
+of $x$ and the @{term Init} operation and @{term \<E>arley} function, and the fact that @{term "Init \<G> \<subseteq> Earley k \<G> \<omega>"}, 
+we have @{term "x \<in> \<E>arley \<G> \<omega>"}, moreover we have @{term "partially_completed |\<omega>| \<G> \<omega> (\<E>arley \<G> \<omega>) (\<lambda>_. True)"}
+using lemma @{thm[source] partially_completed_\<E>arley} and assumption @{term "wf_\<G> \<G>"}, and thus have
+@{term "Item (\<SS> \<G>,\<alpha>) |\<alpha>| 0 |\<omega>| \<in> \<E>arley \<G> \<omega>"} by lemmas @{thm[source] partially_completed_upto} and
+@{thm[source] wf_\<E>arley} and the definition of @{term partially_completed}. The statement @{term "recognizing (\<E>arley \<G> \<omega>) \<G> \<omega>"}
 follows immediately by the definition of @{term recognizing}, @{term is_finished}, and @{term is_complete}.
 
 \end{proof}
 \<close>
 
 corollary correctness_\<E>arley:
-  assumes "wf_cfg cfg"
-  assumes "is_sentence cfg \<omega>"
-  shows "recognizing (\<E>arley cfg inp) cfg \<omega> \<longleftrightarrow> derives cfg [\<SS> cfg] \<omega>"
+  assumes "wf_\<G> \<G>"
+  assumes "is_sentence \<G> \<omega>"
+  shows "recognizing (\<E>arley \<G> \<omega>) \<G> \<omega> \<longleftrightarrow> \<G> \<turnstile> [\<SS> \<G>] \<Rightarrow>\<^sup>* \<omega>"
 (*<*)
   sorry
 (*>*)
@@ -988,17 +1025,17 @@ section \<open>Finiteness\<close>
 text\<open>At last, we prove that the set of Earley items is finite. In Chapter \ref{chap:04}
 we are using this result to prove the termination of an executable version of the algorithm.
 
-Since @{term "\<E>arley cfg \<omega>"} only generates well-formed items (lemma @{thm[source] wf_\<E>arley}) it suffices
+Since @{term "\<E>arley \<G> \<omega>"} only generates well-formed items (lemma @{thm[source] wf_\<E>arley}) it suffices
 to prove that there only exists a finite number of well-formed items. Define 
-  $$@{term "T = (set (\<RR> cfg) \<times> {0::nat..m} \<times> {0..length \<omega>} \<times> {0..length \<omega>}) "} $$
-where @{term "m = Max { length (rule_body r) | r. r \<in> set (\<RR> cfg) }"}. The set $T$ is finite since there
+  $$@{term "T = (set (\<RR> \<G>) \<times> {0::nat..m} \<times> {0..|\<omega>|} \<times> {0..|\<omega>| }) "} $$
+where @{term "m = Max { |rule_body r| | r. r \<in> set (\<RR> \<G>) }"}. The set $T$ is finite since there
 exists only a finite number of production rules and
-@{term "{ x | x. wf_item cfg \<omega> x }"} is a subset of mapping the @{term Item} constructor over $T$ (strictly speaking
+@{term "{ x | x. wf_item \<G> \<omega> x }"} is a subset of mapping the @{term Item} constructor over $T$ (strictly speaking
 we need to first unpack the quadruple).
 \<close>
 
 lemma finiteness_UNIV_wf_item:
-  shows "finite { x | x. wf_item cfg \<omega> x }"
+  shows "finite { x | x. wf_item \<G> \<omega> x }"
 (*<*)
   sorry
 (*>*)
@@ -1006,7 +1043,7 @@ lemma finiteness_UNIV_wf_item:
 text\<open>\<close>
 
 theorem finiteness:
-  shows "finite (\<E>arley cfg \<omega>)"
+  shows "finite (\<E>arley \<G> \<omega>)"
 (*<*)
   sorry
 (*>*)
