MyLaTeXSugar.thy
@@ -51,13 +51,15 @@ notation (latex)
 *)
 
 (* length *)
+(*
 notation (latex output)
   length  ("|_|")
+*)
 
 (* nth *)
 (*
 notation (latex output)
-  nth  ("_\<^latex>\<open>\\ensuremath{_{[\\mathit{\<close>_\<^latex>\<open>}]}}\<close>" [1000,0] 1000)
+  nth  ("_\<^latex>\<open>[\<close>_\<^latex>\<open>]\<close>" [1000,0] 1000)
 *)
 
 (* DUMMY *)
